VeriSkel/Env.v
@@ -4,10 +4,12 @@ Require Import PHeap.
 Section Environment.
   Definition Env (A B : Type) (eqt : eq_type A) := A -> B.
   
-  Definition upd {A B eqt} (env : Env A B eqt) x v : Env A B eqt :=
+  Definition upd {A B} `{eqt : eq_type A} (env : Env A B eqt) x v : Env A B eqt :=
     fun y => if eq_dec x y then v else env y.
-  Definition upd_opt {A B eqt} (env : Env A (option B) eqt) x v : Env A (option B) eqt :=
+  Definition upd_opt {A B} `{eqt : eq_type A} (env : Env A (option B) eqt) x v : Env A (option B) eqt :=
     fun y => if eq_dec x y then Some v else env y.
-  Definition emp_opt {A B eqt} : Env A (option B) eqt := fun (_ : A) => @None B.
-  Definition emp_def {A B eqt} (d : B) : Env A B eqt := fun (_ : A) => d.
+  Definition emp_opt {A B} `{eqt : eq_type A} : Env A (option B) eqt := fun (_ : A) => @None B.
+  Definition emp_def {A B} `{eqt : eq_type A} (d : B) : Env A B eqt := fun (_ : A) => d.
+
+  Definition env_map {A B C} `{eqt : eq_type A} f (env : Env A B eqt) : Env A C eqt := fun y => f (env y).
 End Environment.
